Coq is segfaulting.

MirrorCharge!/src/MirrorCharge/Imp/Bench_Mem.v
@@ -5,6 +5,14 @@ Require Import MirrorCharge.Imp.SymEvalLemmas.
 Require MirrorCharge.Imp.STacCancel.
 Require Import MirrorCharge.Imp.Syntax.
 
+Local Existing Instance SS.
+Local Existing Instance SU.
+Local Existing Instance RSym_ilfunc.
+Local Existing Instance RS.
+Local Existing Instance RSOk.
+Local Existing Instance Expr_expr.
+Local Existing Instance ExprOk_expr.
+
 Definition entailment_tac : imp_tac := THEN SIMPLIFY (runOnGoals STacCancel.stac_cancel).
 Definition simplify_tac : imp_tac := SIMPLIFY.
 
@@ -28,7 +36,7 @@ Definition EAPPLY_THEN_1 a (side : imp_tac) (b : imp_tacK) : imp_tac :=
                                                 end))))).
 
 Definition sym_eval_mem (n : nat) : imp_tac :=
-  REC_N n (fun rec : imp_tac =>
+  REC n (fun rec : imp_tac =>
            let rec := THEN simplify_tac (runOnGoals rec) in
            FIRST (   EAPPLY_THEN SeqA_lemma rec
                   :: EAPPLY_THEN Assign_seq_lemma rec
@@ -44,7 +52,129 @@ Definition sym_eval_mem (n : nat) : imp_tac :=
                   :: nil))
       IDTAC.
 
+Lemma runTacK_sound : forall t, rtacK_sound t -> rtac_sound (runTacK t).
+Proof.
+  unfold rtacK_sound, rtac_sound, runTacK, rtac_spec, rtacK_spec. intros.
+  eapply H; eauto.
+Qed.
 
+Lemma simplify_tac_sound : rtac_sound simplify_tac.
+apply SIMPLIFY_sound.
+Qed.
+
+Lemma entailment_tac_sound : rtac_sound entailment_tac.
+Admitted.
+
+Lemma entailment_tac_solve_sound : rtac_sound entailment_tac_solve.
+apply SOLVE_sound. apply entailment_tac_sound.
+Qed.
+
+
+Ltac rtac_derive_soundness' tac tacK lems :=
+  let lems := (auto ; lems) in
+  let rec rtac :=
+      try first [ simple eapply IDTAC_sound
+                | simple eapply FAIL_sound
+                | simple eapply FIRST_sound ; Forall_rtac
+                | simple eapply SOLVE_sound ; rtac
+                | simple eapply THEN_sound ;
+                  [ rtac
+                  | rtacK ]
+                | simple eapply TRY_sound ; rtac
+                | simple eapply REPEAT_sound ; rtac
+                | simple eapply REC_sound ; intros; rtac
+                | simple eapply AT_GOAL_sound ; [ intros ; rtac ]
+                | simple eapply APPLY_sound ; [ lems ]
+                | simple eapply EAPPLY_sound ; [ lems ]
+                | simple eapply runTacK_sound ; [ rtacK ]
+                | solve [ eauto ]
+                | tac rtac rtacK lems
+                ]
+  with rtacK :=
+      try first [ simple eapply runOnGoals_sound ; rtac
+                | simple eapply MINIFY_sound
+                | simple eapply THENK_sound ; [ try rtacK | try rtacK ]
+                | solve [ eauto ]
+                | tacK rtac rtacK lems
+                | eapply runOnGoals_sound ; rtac
+                ]
+  with Forall_rtac :=
+      repeat first [ eapply Forall_nil
+                   | eapply Forall_cons ;
+                     [ rtac
+                     | Forall_rtac ]
+                   | solve [ eauto ] ]
+  in
+  match goal with
+    | |- rtac_sound _ => rtac
+    | |- rtacK_sound _ => rtacK
+    | |- Forall rtac_sound _ => Forall_rtac
+  end.
+
+Ltac rtac_derive_soundness_default :=
+  rtac_derive_soundness' ltac:(fun rtac _ _ =>
+                                 match goal with
+                                   | |- rtac_sound match ?X with _ => _ end =>
+                                     destruct X; rtac
+                                 end)
+                         ltac:(fun _ _ _ => fail)
+                         ltac:(idtac).
+
+Lemma EAPPLY_THEN_sound : forall lem tac,
+                            Lemma.lemmaD (exprD'_typ0 (T:=Prop)) nil nil lem -> rtac_sound tac -> 
+                            rtac_sound (EAPPLY_THEN lem tac).
+Proof. intros; unfold EAPPLY_THEN.
+       rtac_derive_soundness_default.
+Qed.
+
+Lemma EAPPLY_THEN_1_sound
+: forall lem tac1 tac2,
+    Lemma.lemmaD (exprD'_typ0 (T:=Prop)) nil nil lem ->
+    rtac_sound tac1 -> rtacK_sound tac2 ->
+    rtac_sound (EAPPLY_THEN_1 lem tac1 tac2).
+Proof. intros; unfold EAPPLY_THEN_1.
+       rtac_derive_soundness_default.
+Qed.
+
+Ltac one_of lems :=
+  match lems with
+    | (?X,?Y) => first [ one_of X | one_of Y ]
+    | _ => exact lems
+  end.
+
+Ltac red_lemma :=
+  unfold Lemma.lemmaD, Lemma.lemmaD'; simpl;
+  unfold ExprDsimul.ExprDenote.exprT_App, ExprDsimul.ExprDenote.exprT_Abs, exprT_Inj, SymEnv.funcD, ExprDsimul.ExprDenote.Rcast_val, ExprDsimul.ExprDenote.Rcast; simpl.
+
+Hint Immediate Imp.SeqA_rule
+     Imp.Assign_seq_rule Imp.Assign_tail_rule
+     Imp.Read_seq_rule Imp.Read_tail_rule
+     Imp.Write_seq_rule Imp.Write_tail_rule : the_hints.
+
+Ltac rtac_derive_soundness_with :=
+  rtac_derive_soundness' ltac:(fun rtac rtacK lem =>
+                                 first [ eapply EAPPLY_THEN_sound ; [ lem | rtac ]
+                                       | eapply EAPPLY_THEN_1_sound ; [ lem | rtac | rtacK ]
+                                       | eapply simplify_tac_sound
+                                       | eapply entailment_tac_sound
+                                       | eapply entailment_tac_solve_sound
+                                       | match goal with
+                                           | |- rtac_sound match ?X with _ => _ end =>
+                                             destruct X; rtac
+                                         end ])
+                         ltac:(fun _ _ => fail)
+                         ltac:(idtac "lemma"; try solve [ red_lemma; eauto with the_hints ]).
+
+Goal forall n, rtac_sound (sym_eval_mem n).
+intros. unfold sym_eval_mem.
+rtac_derive_soundness_with.
+exact Imp.Read_seq_rule.
+exact Imp.Skip_seq_rule.
+exact Imp.Assert_seq_rule.
+exact Imp.Read_tail_rule.
+exact Imp.Skip_tail_rule.
+exact Imp.Assert_tail_rule.
+Qed.
 
 Definition Prove P c Q :=
   App
@@ -67,6 +197,7 @@ Fixpoint adds_syn (n : nat) :=
     | S n => Syntax.mkSeq (Syntax.mkAssign (Syntax.fVar "x") (Syntax.fVar "x")) (adds_syn n)
   end%string.
 
+(*
 Time Eval vm_compute in
     let tus := nil in
     let tvs := nil in
@@ -85,6 +216,7 @@ Time Eval vm_compute in
     let tvs := nil in
     let goal := Prove (Syntax.ltrue Syntax.tyLProp) (adds_syn n) (Syntax.ltrue Syntax.tyLProp) in
     runImpTac tus tvs goal (sym_eval_mem n).
+*)
 
 Fixpoint adds (n : nat) :=
   match n with
@@ -94,7 +226,7 @@ Fixpoint adds (n : nat) :=
 
 Goal @ILogic.lentails Imp.SProp Imp.ILogicOps_SProp (@ILogic.ltrue Imp.SProp Imp.ILogicOps_SProp)
      (Imp.triple (@ILogic.ltrue Imp.lprop Imp.ILogicOps_lprop)
-        (adds 10)
+        (adds 1)
         (@ILogic.ltrue Imp.lprop Imp.ILogicOps_lprop)).
 unfold adds.
 match goal with
@@ -103,4 +235,18 @@ match goal with
         pose g
     in
     reify_expr Reify.reify_imp k [ True ] [ goal ]
+end.
+
+
+Check rtac_Solved_closed_soundness.
+pose (runRtac typ (expr typ func) nil nil e (sym_eval_mem 2)).
+assert (r = Fail).
+vm_compute.
+vm_compute in r.
+let result := constr:(runRtac typ (expr typ func) nil nil e (sym_eval_mem 100)) in
+let resultV := eval vm_compute in result in
+idtac resultV ;
+match resultV with
+| Solved _ => idtac "Solved"
+| More_ _ _ => idtac "More_"
 end.
