MirrorCharge!/src/MirrorCharge/Imp/ImpTac.v
@@ -14,7 +14,9 @@ Local Existing Instance SS.
 Local Existing Instance SU.
 Local Existing Instance RSym_ilfunc.
 Local Existing Instance RS.
+Local Existing Instance RSOk.
 Local Existing Instance Expr_expr.
+Local Existing Instance ExprOk_expr.
 
 Definition imp_tac := rtac typ (expr typ func).
 Definition imp_tacK := rtacK typ (expr typ func).
@@ -27,6 +29,17 @@ Definition EAPPLY lem : imp_tac :=
                  lem)
        (@MINIFY _ _ _).
 
+Theorem EAPPLY_sound
+: forall lem,
+    Lemma.lemmaD (exprD'_typ0 (T:=Prop)) nil nil lem ->
+    rtac_sound (EAPPLY lem).
+Proof.
+  intros. eapply THEN_sound.
+  - eapply EAPPLY_sound; eauto with typeclass_instances.
+    admit. admit.
+  - eapply MINIFY_sound.
+Qed.
+
 Definition APPLY lem : imp_tac :=
   THEN (@APPLY typ (expr typ func) _ _ _ _ ExprLift.vars_to_uvars
                 (fun subst S_subst SU tus tvs n e1 e2 s t =>
@@ -35,8 +48,27 @@ Definition APPLY lem : imp_tac :=
                 lem)
        (@MINIFY _ _ _).
 
+Theorem APPLY_sound
+: forall lem,
+    Lemma.lemmaD (exprD'_typ0 (T:=Prop)) nil nil lem ->
+    rtac_sound (EAPPLY lem).
+Proof.
+  intros. eapply THEN_sound.
+  - eapply APPLY_sound; eauto with typeclass_instances.
+    admit. admit.
+  - eapply MINIFY_sound.
+Qed.
+
 Definition SIMPLIFY : imp_tac :=
   SIMPLIFY (fun _ _ _ _ => beta_all (idred simplify)).
+
+Theorem SIMPLIFY_sound : rtac_sound SIMPLIFY.
+Proof.
+  eapply SIMPLIFY_sound. intros.
+  unfold Ctx.propD, exprD'_typ0 in *.
+  Require Import ExtLib.Tactics.
+  forward. inv_all. subst.
+Admitted.
 
 Definition runOnGoals (t : imp_tac) : imp_tacK := runOnGoals t.
 Coercion runOnGoals : imp_tac >-> imp_tacK.
